partially verified donordb

projectVampire/blood.dfy
@@ -9,17 +9,27 @@ datatype Blood_types = A | B | AB
 
 class Blood{
     var state: int;
+    var hour: int;
+    var minute:int;
+    var day:int;
     var blood_type: Blood_types;
 
     predicate Valid()
     reads this
     {0<=state<=5}
 
-    constructor ()
+    constructor (dayin:int,hourin:int,minutein:int)
     modifies this
+    requires 0<=dayin && 0<=hourin<=23 && 0<=minutein<=59
+    ensures 0<=day && 0<=hour<=23 && 0<=minute<=59
     ensures Valid();
     ensures state == 0;
-    {state := 0;}
+    {
+        hour:=hourin;
+        day:=dayin;
+        minute:=minutein;
+        state := 0;
+    }
 
     method verify(determined_type:Blood_types)
     modifies this
