projectVampire/donordb.dfy
@@ -1,7 +1,59 @@
+#include blood.dfy
+
 class donor
 {
     var last_donation: int // Day of last donation as integer since system instantiation
 
-    method collectBlood()
-    {}
+    constructor ()
+    modifies this
+    ensures last_donation==-7
+    {last_donation:=-7;}
+
+
+    predicate donation_allowed(day:int)
+    reads this
+    {day - last_donation >= 7}
+
+    method collectBlood(day:int,hour:int,minute:int) returns (blood:Blood)
+    modifies this
+    requires donation_allowed(day)
+    requires 0<=day && 0<=hour<=23 && 0<=minute<=59
+    ensures last_donation == day
+    {
+        last_donation:=day;
+        var blud := new Blood(day,hour,minute);
+        return blud;
+    }
+}
+
+
+
+// Date in Dafny?
+method get_hour() returns (hour:int)
+ensures 0<=hour<=23
+{
+    return 14;
+}
+
+
+method get_day() returns (day:int)
+ensures 0<=day
+{
+    return 10;
+}
+
+method get_minute() returns (minute:int)
+ensures 0<=minute<=59
+{
+    return 36;
+}
+
+method Test()
+{
+    var doner := new Donor();
+
+    var blud_1 := doner.collectBlood(1,1,1);
+    assert !doner.donation_allowed(2);
+    assert doner.donation_allowed(17);
+    // doner.collectBlood(2,2,2);
 }
